cclc

coq/cclc/clc_subtype.v
@@ -14,7 +14,11 @@ Inductive sub1 : term -> term -> Prop :=
   sub1 (s @ l1) (s @ l2)
 | sub1_pi A B1 B2 s t : 
   sub1 B1 B2 -> 
-  sub1 (Pi A B1 s t) (Pi A B2 s t).
+  sub1 (Pi A B1 s t) (Pi A B2 s t)
+| sub1_sigma A1 A2 B1 B2 s r t :
+  sub1 A1 A2 ->
+  sub1 B1 B2 ->
+  sub1 (Sigma A1 B1 s r t) (Sigma A2 B2 s r t).
 
 CoInductive sub (A B : term) : Prop :=
 | SubI A' B' : 
@@ -41,7 +45,8 @@ Proof with eauto 6 using sub1, sub1_sub, sub1_conv, conv_sub1.
   move=> sb. elim: sb C D => {A B}
     [ A C D 
     | s l1 l2 leq C D conv sb
-    | A B1 B2 s t sb1 ih C D conv sb2 ]...
+    | A B1 B2 s t sb1 ih C D conv sb2 
+    | A1 A2 B1 B2 s r t sb1 ih1 sb2 ih2 C D conv sb3 ]...
   inv sb; try (exfalso; solve_conv)...
     move: conv => /sort_inj [->eq].
     apply: sub_sort. subst.
@@ -51,8 +56,18 @@ Proof with eauto 6 using sub1, sub1_sub, sub1_conv, conv_sub1.
     move: (ih _ _ conv2 H) => {ih} sub. inv sub.
     apply: SubI. 
     apply sub1_pi with (s := s0) (t := t0)... 
-    exact: conv_pi... 
+    exact: conv_pi. 
     exact: conv_pi.
+  inv sb3; try (exfalso; solve_conv)...
+    move: conv => /sigma_inj[conv1[conv2[->[->->]]]].
+    move: (ih1 _ _ conv1 H)=>{ih1}sub1.
+    move: (ih2 _ _ conv2 H0)=>{ih2}sub2.
+    inv sub1. inv sub2.
+    apply: SubI.
+    apply sub1_sigma with (s := s0) (r := r0) (t := t0).
+    exact: H1. exact: H4.
+    exact: conv_sigma.
+    exact: conv_sigma.
 Qed.
 
 Lemma sub_trans B A C :
@@ -73,6 +88,7 @@ Proof.
     inv l=> //.
   move=> s l0 l3 leq /sort_inj[->->]/sort_inj[<-<-]=> //.
   move=> *. exfalso; solve_conv.
+  move=> *. exfalso; solve_conv.
 Qed.
 
 Lemma sub_pi_inv A1 A2 s1 s2 t1 t2 B1 B2 :
@@ -89,6 +105,24 @@ Proof.
   move=> A B0 B3 s t sb /pi_inj[c1[c2[<-<-]]]/pi_inj[c3[c4[->->]]]. 
     firstorder.
     exact: conv_trans c3. exact: SubI sb c2 c4.
+  move=> *. exfalso; solve_conv.
+Qed.
+
+Lemma sub_sigma_inv A1 A2 B1 B2 p1 p2 q1 q2 s1 s2 :
+  Sigma A1 B1 p1 q1 s1 <: Sigma A2 B2 p2 q2 s2 -> 
+  A1 <: A2 /\ B1 <: B2 /\ p1 = p2 /\ q1 = q2 /\ s1 = s2.
+Proof.
+  move=> [A' B' []].
+  move=> C c1 c2. 
+    have{c1 c2}/sigma_inj[c1[c2[->[->->]]]]: 
+      Sigma A1 B1 p1 q1 s1 === Sigma A2 B2 p2 q2 s2.
+    exact: conv_trans c2.
+    firstorder=>//. exact: conv_sub. exact: conv_sub.
+  move=> *. exfalso; solve_conv.
+  move=> *. exfalso; solve_conv.
+  move=>A A0 B0 B3 s r t sb1 sb2
+    /sigma_inj[c1[c2[<-[<-<-]]]]/sigma_inj[c3 [c4 [->[->->]]]]. 
+    firstorder. exact: SubI sb1 c1 c3. exact: SubI sb2 c2 c4.
 Qed.
 
 Lemma sub1_subst σ A B : sub1 A B -> sub1 A.[σ] B.[σ].
