coq/cclc/clc_ast.v
@@ -7,11 +7,17 @@ Unset Strict Implicit.
 Unset Printing Implicit Defensive.
 
 Inductive term : Type :=
-| Var (x : var)
-| Sort (s : sort) (l : nat)
-| Pi (A : term) (B : {bind term}) (s t : sort)
-| Lam (A : term) (B : {bind term}) (s t : sort)
-| App (m n : term).
+| Var    (x : var)
+| Sort   (s : sort) (l : nat)
+| Pi     (A : term) (B : {bind term}) (s t : sort)
+| Lam    (A : term) (B : {bind term}) (s t : sort)
+| App    (m n : term)
+| Unit
+| It
+| Sigma  (A : term) (B : {bind term}) (s r t : sort)
+| Pair   (m n : term)
+| LetIn1 (m n : term)
+| LetIn2 (m : term) (n : {bind 2 of term}).
 
 Notation "s @ l" := (Sort s l) (at level 30).
 
@@ -42,6 +48,34 @@ Inductive step : term -> term -> Prop :=
 | step_appR m n n' :
   n ~> n' ->
   App m n ~> App m n'
+| step_sigmaL A A' B s r t :
+  A ~> A' ->
+  Sigma A B s r t ~> Sigma A' B s r t
+| step_sigmaR A B B' s r t :
+  B ~> B' ->
+  Sigma A B s r t ~> Sigma A B' s r t
+| step_pairL m m' n :
+  m ~> m' ->
+  Pair m n ~> Pair m' n
+| step_pairR m n n' :
+  n ~> n' ->
+  Pair m n ~> Pair m n'
+| step_letin1L m m' n :
+  m ~> m' ->
+  LetIn1 m n ~> LetIn1 m' n
+| step_letin1R m n n' :
+  n ~> n' ->
+  LetIn1 m n ~> LetIn1 m n'
+| step_iota1 n :
+  LetIn1 It n ~> n
+| step_letin2L m m' n :
+  m ~> m' ->
+  LetIn2 m n ~> LetIn2 m' n
+| step_letin2R m n n' :
+  n ~> n' ->
+  LetIn2 m n ~> LetIn2 m n'
+| step_iota2 m1 m2 n :
+  LetIn2 (Pair m1 m2) n ~> n.[m2,m1/]
 where "m ~> n" := (step m n).
 
 Notation red := (star step).
